
\titlebox{language}{
\begin{mathpar}
e ::= x | exp

exp ::= \lambda(x, \ ..., \ x). \ e \ | \ e(e, \ ..., \ e) \ | \ e; e \ | \ x \leftarrow e
\end{mathpar}
}

\titlebox{Syntaxe des types, des contraintes et des environnements}{
\begin{mathpar}
\Gamma ::= x : \sigma, \ \Gamma \ | \alpha, \Gamma | \alpha_c, \Gamma | \ \emptyset

H ::= \exists x :_n \tau, \ H \ | \ \alpha_c, \ H \ | \ \emptyset

U ::= x : \tau, \ U \ | \ \emptyset

\sigma ::= \forall \alpha. \ \sigma \ | \forall \alpha_c . \ \sigma \ | \ \tau

\tau ::= (\tau, ..., \tau) \rightarrow_{[c]} \tau \ | \ \alpha

c ::= \exists x :_n \tau \ | \ c \land c \ | \ \alpha_c

\end{mathpar}
}

\titlebox{Rules (1)}{
\begin{mathpar}
  \def \RightTirName #1{\rm\hbox {\hskip 1ex (#1)}}
  \inferrule*[Left=Assign]
             {
               \Gamma, U, H \vdash_{false, n} e : \sigma, \ \Gamma', U' \\
               \forall (x : \tau_x) \in U'. (x : \sigma, \ \Gamma'), \emptyset, H \vdash_{false, n} x : \tau_x, (x : \sigma, \ \Gamma'), \emptyset
             }
             { \Gamma, U, H \vdash_{false, n} x = e : \sigma, (x : \sigma, \ \Gamma'), U' }

  \inferrule*[Left=Seq]
             { \Gamma, U, H \vdash_{b,n} e_1 : \tau_1, \Gamma_1, U_1 \\ \Gamma_1, U_1, H \vdash_{b,n} e_2 : \tau_2, \Gamma_2, U_2 }
             { \Gamma, U, H \vdash_{b,n} e_1; e_2 : \tau_2, \Gamma_2, U_2 }

  \inferrule* [Left=Abs]
              {
                (x_0 : \tau_0, ..., x_n : \tau_n), \emptyset, H_f \vdash_{false,n+1} e : \tau_r, \Gamma_f, U_f  \\
                H_f \Rightarrow_n c_f  \\
                \tau_{r'} = simpl_{n+1}(\Gamma_f \cup ftv(H_f) \cup fcv(H_f), \tau_r) \\
                WF((\tau_0, ..., \tau_n) \rightarrow_{[c_f]} \tau_{r'})
              }
              {
                \Gamma, U, H \vdash_{b,n} \lambda (x_0, ... , x_n). e : (\tau_0, ..., \tau_n) \rightarrow_{[c_f]} \tau_{r'}, \ \Gamma, U
              }

  \inferrule* [Left=App]
              {
                \Gamma, U, H \vdash_{b,n} e_f : (\tau_0, ..., \tau_m) \rightarrow_{[c_f]} \tau_r, \Gamma', U_f \\
                \Gamma', \emptyset, H \vdash_{true,n} e_0 : \tau_0, \Gamma', U_0  \\ ... \\
                \Gamma', \emptyset, H \vdash_{true,n} e_n : \tau_n, \Gamma', U_n \\
                H \vdash_n simpl_n(\Gamma' \cup ftv(H) \cup fcv(H), c_f)
              }
              {
                \Gamma, U, H \vdash_{b,n} e_f (e_0, ..., e_n) : \tau_r, \ \Gamma', U_f \cup U_0 \cup ... \cup U_n
              }

\end{mathpar}


\begin{mathpar}
  \inferrule* [Left=Var]
              { }
              { \Gamma, U, H \vdash_{false,n} x : \Gamma(x), \Gamma, U }


  \inferrule* [Left=Var, Right={$\#\forall(\Gamma(x)) = 0$}]
              { }
              { \Gamma, U, H \vdash_{true,n} x : \Gamma(x), \Gamma, (x : \Gamma(x)) \cup U }


  \inferrule* [Left=Var, Right=$\#\forall(\Gamma(x)) > 0$]
              { }
              { \Gamma, U, H \vdash_{true,n} x : \Gamma(x), \Gamma, U }
\end{mathpar}

\begin{mathpar}


  \inferrule* [Left=FreeVar]
              { x \notin \Gamma \\ H \vdash \exists x :_{n-1} \tau \\ WF(\tau) }
              { \Gamma, U, H \vdash_{false,n} x : \tau, \Gamma, U }


  \inferrule* [Left=FreeVar]
              { x \notin \Gamma \\ H \vdash \exists x :_{n-1} \tau \\ WF(\tau) }
              { \Gamma, U, H \vdash_{true,n} x : \tau, \Gamma, (x : \tau) \cup U }
\end{mathpar}


}

\titlebox{Règles (2)}{
\begin{mathpar}
  \inferrule*[Left=Gen]
             { \Gamma, U, H \vdash_{b,n} e : \sigma, \Gamma', U' \\
               \alpha \notin ftv(\Gamma) \cup ftv(H) }
             { \Gamma, U, H \vdash_{b,n} e : \forall \alpha. \sigma, \Gamma', U' }
\\
  \inferrule*[Left=GenC]
             { \Gamma, U, H \vdash_{b,n} e : \sigma, \Gamma', U' \\
               \alpha_c \notin fcv(\Gamma) \cup fcv(H)}
             { \Gamma, U, H \vdash_{b,n} e : \forall \alpha_c. \sigma, \Gamma', U' }
\end{mathpar}

\begin{mathpar}
  \inferrule*[Left=Inst]
             { \Gamma, U, H \vdash_{false,n} e : \forall \alpha. \sigma, \ \Gamma', U' }
             { \Gamma, U, H \vdash_{false,n} e : [\alpha \Rightarrow \tau] \sigma, \ \Gamma', U' }
\\
  \inferrule*[Left=InstVar, Right={$\#\forall(\sigma) = 0$}]
             { \Gamma, U, H \vdash_{true,n} x : \forall \alpha. \sigma, \ \Gamma, U
             }
             { \Gamma, U, H \vdash_{true,n} x : [\alpha \Rightarrow \tau] \sigma, \ \Gamma, \ (x : [\alpha \Rightarrow \tau] \sigma) \cup U }
\\
  \inferrule*[Left=InstVar, Right={$\#\forall(\sigma) > 0$}]
             { \Gamma, U, H \vdash_{true,n} x : \forall \alpha. \sigma, \ \Gamma, U
             }
             { \Gamma, U, H \vdash_{true,n} x : [\alpha \Rightarrow \tau] \sigma, \ \Gamma, U }
\\
  \inferrule*[Left=InstExp]
             { \Gamma, U, H \vdash_{true,n} exp : \forall \alpha. \sigma, \ \Gamma, U'
             }
             { \Gamma, U, H \vdash_{true,n} exp : [\alpha \Rightarrow \tau] \sigma, \ \Gamma, U' }

\end{mathpar}

\begin{mathpar}
  \inferrule*[Left=InstC]
             { \Gamma, U, H \vdash_{false,n} e : \forall \alpha_c. \sigma, \Gamma', U' }
             { \Gamma, U, H \vdash_{false,n} e : [\alpha_c \Rightarrow c] \sigma, \Gamma', U' }
\\
  \inferrule*[Left=InstCVar, Right={$\#\forall(\sigma) = 0$}]
             { \Gamma, U, H \vdash_{true,n} x : \forall \alpha_c. \sigma, \Gamma, U
             }
             { \Gamma, U, H \vdash_{true,n} x : [\alpha_c \Rightarrow c] \sigma, \Gamma, \ (x : [\alpha_c \Rightarrow c] \sigma) \cup U }
\\
  \inferrule*[Left=InstCVar, Right={$\#\forall(\sigma) > 0$}]
             { \Gamma, U, H \vdash_{true,n} x : \forall \alpha_c. \sigma, \Gamma, U
             }
             { \Gamma, U, H \vdash_{true,n} x : [\alpha_c \Rightarrow c] \sigma, \Gamma, U }
\\
  \inferrule*[Left=InstCExp]
             { \Gamma, U, H \vdash_{true,n} exp : \forall \alpha_c. \sigma, \Gamma, U' }
             { \Gamma, U, H \vdash_{true,n} exp : [\alpha_c \Rightarrow c] \sigma, \Gamma, U' }
\end{mathpar}
}




\titlebox{WF}{
\begin{mathpar}
  \inferrule*
      { }
      { WF(\alpha) }

  \inferrule*
      { WF(\tau_r) \\ WF(c) \\ wf(\tau_0) \\ ... \\ wf(\tau_n) }
      { WF((\tau_0, ..., \tau_n) \rightarrow_{[c]}\tau_r) }

  \inferrule*
      { }
      { WF(\alpha_c) }

  \inferrule*
      { WF(c_1) \\ WF(c_2) }
      { WF(c_1 \land c_2) }

  \inferrule*
      { wf(\tau) }
      { WF(\exists x : \tau) }

  \inferrule*
      { }
      { wf(\alpha) }

  \inferrule*
      { wf(\tau_0) \\ ... \\ wf(\tau_n) \\ wf(\tau_r) }
      { wf((\tau_0, ..., \tau_n) \rightarrow_{[\alpha_c]}\tau_r) }

\end{mathpar}
}


\titlebox{simpl}{
\begin{mathpar}


  \inferrule*
      { }
      { simpl_n(\Gamma, \alpha) \Rightarrow \alpha }

   \inferrule*
      {  }
      { simpl_n(\Gamma, \alpha_c) \Rightarrow \alpha_c }

  \inferrule*
      { simpl_n(\Gamma, \tau_r) \Rightarrow \tau_r' \\ simpl_n(\Gamma, c) \Rightarrow c' }
      { simpl_n(\Gamma, (\tau_0, ..., \tau_n) \rightarrow_{[c]}\tau_r) \Rightarrow (\tau_0, ..., \tau_n) \rightarrow_{[c']}\tau_r' }

   \inferrule*
      { simpl_n(\Gamma, c_1) \Rightarrow c_3 \\ simpl_n(\Gamma, c_2) \Rightarrow c_4 }
      { simpl_n(\Gamma, c_1 \land c_2) \Rightarrow c_3 \land c_4 }

   \inferrule*
      { x \notin \Gamma}
      { simpl_n(\Gamma, \exists x :_{n} \tau) \Rightarrow \exists x :_{n-1} \tau }

   \inferrule*
      {  }
      { simpl_n(\Gamma, \exists x :_{n-1} \tau) \Rightarrow \exists x :_{n-1} \tau }




   \inferrule* [Right={$\alpha_c \ chosen \ fresh$}]
      {  \Gamma, \emptyset, \emptyset \vdash_{false, n} x : \tau, \Gamma, \emptyset }
      { simpl_n(\Gamma, \exists x :_n \tau) \Rightarrow \alpha_c }



\end{mathpar}
}


\titlebox{Transformation des hypothèses vers les contraintes}{
\begin{mathpar}
  \inferrule*[Right={$\alpha_c \ chosen \ fresh$}]
      {  }
      { \emptyset \Rightarrow_n \alpha_c }


  \inferrule*
      {  H \Rightarrow_n c }
      { (\exists x :_n \tau), H \Rightarrow_n (\exists x :_n \tau) \land c }

  \inferrule*
      {  }
      { \alpha_c \Rightarrow_n \alpha_c }

\end{mathpar}
} 

\titlebox{Satisfaction des contraintes}{
\begin{mathpar}
  \inferrule*[Right={$n > 0$}]
      { \alpha_c \in H }
      { H \vdash_n \alpha_c }

  \inferrule*
      {  }
      { H \vdash_0 \alpha_c }

  \inferrule*
      { (\exists x :_n \tau) \in H }
      { H \vdash_n \exists x :_n \tau }

  \inferrule*
      { H \vdash_n c_1 \\ H \vdash_n c_2 }
      { H \vdash_n c_1 \land c_2 }

\end{mathpar}
} 
